Make the compiler, and start the compiler verification

VeriSkel/Lang.v
@@ -3,72 +3,24 @@ Require Import Vector.
 Require Import List.
 Require Import ZArith.
 Require Import GPUCSL.
+Require Import LibTactics.
 Definition name := string. 
+
+(* general enviroment *)
+Section Environment.
+  Definition Env (A B : Type) (eqt : eq_type A) := A -> B.
+  
+  Definition upd {A B eqt} (env : Env A B eqt) x v : Env A B eqt :=
+    fun y => if eq_dec x y then v else env y.
+  Definition upd_opt {A B eqt} (env : Env A (option B) eqt) x v : Env A (option B) eqt :=
+    fun y => if eq_dec x y then Some v else env y.
+  Definition emp_opt {A B eqt} : Env A (option B) eqt := fun (_ : A) => @None B.
+  Definition emp_def {A B eqt} (d : B) : Env A B eqt := fun (_ : A) => d.
+End Environment.
+
+(* variables for scalar expressions/arrays *)
 Inductive varE : Set := VarE (name : string).
 Inductive varA : Set := VarA (name : string).
-
-Inductive SOp : Set := Eplus | Emax | BEq | Blt.
-
-Inductive SExp :=
-| EVar (x : varE)
-| Enum (x : Z)
-| ELet (x : varE) (e e' : SExp)
-| EBin (op : SOp) (e1 e2 : SExp)
-| EA (x : varA) (e : SExp)
-| EPrj (e : SExp) (i : nat)
-| ECons (es : list SExp)
-| EIf (e e' e'' : SExp).
-
-Lemma SExp_ind' : forall P : SExp -> Prop,
-    (forall x : varE, P (EVar x)) ->
-    (forall x : Z, P (Enum x)) ->
-    (forall (x : varE) (e : SExp), P e -> forall e' : SExp, P e' -> P (ELet x e e')) ->
-    (forall (op : SOp) (e1 : SExp), P e1 -> forall e2 : SExp, P e2 -> P (EBin op e1 e2)) ->
-    (forall (x : varA) (e : SExp), P e -> P (EA x e)) ->
-    (forall e : SExp, P e -> forall i : nat, P (EPrj e i)) ->
-    (forall (es : list SExp), List.Forall P es -> P (ECons es)) ->
-    (forall e : SExp, P e -> forall e' : SExp, P e' -> forall e'' : SExp, P e'' -> P (EIf e e' e'')) ->
-    forall e : SExp, P e.
-Proof.
-  intros; revert e.
-  refine (fix rec (e : SExp) := 
-    match e return P e with
-    | EVar x => H _
-    | Enum x => H0 _
-    | ELet x e e' => H1 _ _ (rec _) _ (rec _)
-    | EBin op e1 e2 => H2 _ _ (rec _) _ (rec _)
-    | EA x e => H3 _ _ (rec _)
-    | EPrj e i => H4 _ (rec _) _
-    | ECons es => 
-      let fix rec2 (es : list SExp) : List.Forall P es :=
-          match es return List.Forall P es with
-          | nil => List.Forall_nil _
-          | (e :: es')%list => List.Forall_cons _ (rec e) (rec2 es')
-          end in
-      H5 _ (rec2 es)
-    | EIf e e' e'' => H6 _ (rec _) _ (rec _) _ (rec _)
-    end).
-Qed.
-
-Inductive Func := F (params : list varE) (body : SExp).
-
-Inductive AE :=
-  ALet (va : varA) (sk : name) (fs : list Func) (vas : list varA) (ea : AE)
-| ARet (va : varA).
-
-Inductive SVal : Set :=
-| VB (b : bool) | VZ (n : Z) | VTup (vs : list SVal).
-Record array :=
-  Arr {len : nat; dim : nat; arr : list SVal}.
-
-Definition Env (A B : Type) (eqt : eq_type A) := A -> B.
-
-Definition upd {A B eqt} (env : Env A B eqt) x v : Env A B eqt :=
-  fun y => if eq_dec x y then v else env y.
-Definition upd_opt {A B eqt} (env : Env A (option B) eqt) x v : Env A (option B) eqt :=
-  fun y => if eq_dec x y then Some v else env y.
-Definition emp_opt {A B eqt} : Env A (option B) eqt := fun (_ : A) => @None B.
-Definition emp_def {A B eqt} (d : B) : Env A B eqt := fun (_ : A) => d.
 
 Instance eq_varA : eq_type varA.
 Proof.
@@ -82,9 +34,123 @@ Proof.
   repeat decide equality. 
 Defined.
 
+(* scalar operations *)
+Inductive SOp : Set := Eplus | Emax | BEq | Blt.
+
+(* types of scala expressions *)
+Inductive Typ := TBool | TZ | TTup (typs : list Typ).  
+
+Inductive Forall_rect (A : Type) (P : A -> Type) : list A -> Type :=
+    Forall_r_nil : Forall_rect A P nil
+  | Forall_r_cons : forall (x : A) (l : list A), P x -> Forall_rect A P l -> Forall_rect A P (x :: l).
+
+Lemma STyp_rect' (P : Typ -> Type) (f : P TBool) (f0 : P TZ)
+      (f1 : forall (typs : list Typ), (Forall_rect _ P typs) -> (P (TTup typs))) : forall ty, P ty.
+  refine
+    (let fix rec ty :=
+     match ty as s0 return (P s0) with
+     | TBool => f
+     | TZ => f0
+     | TTup x =>
+       let fix rec (tys : list Typ) :=
+           match tys return Forall_rect _ P tys with
+           | nil => Forall_r_nil _ _
+           | ty :: tys => Forall_r_cons _ _ _ _ _ _
+           end in f1 _ (rec x)
+     end in rec).
+  eauto.
+  eauto.
+Qed.
+
+Lemma STyp_eq_dec (ty1 ty2 : Typ) : {ty1 = ty2} + {ty1 <> ty2}.
+Proof.
+  revert ty2 ty1; apply (STyp_rect' (fun ty => forall ty2, {ty2 = ty} + {ty2 <> ty}));
+  destruct ty2; try first [left; congruence | right; congruence].
+  revert typs0; induction X.
+  - destruct typs0; [left | right]; congruence.
+  - destruct typs0.
+    + right; congruence.
+    + lets [?|?]: (IHX typs0).
+      * lets [?|?]: (p t).
+        inversion e; substs; left; eauto.
+        right; congruence.
+      * right; congruence.
+Defined.
+
+(* scalar expressions *)
+Inductive SExp :=
+| EVar (x : varE) (typ : Typ)
+| Enum (x : Z)
+| ELet (x : varE) (e e' : SExp) (typ : Typ)
+| EBin (op : SOp) (e1 e2 : SExp) (typ : Typ)
+| EA (x : varA) (e : SExp) (typ : Typ)
+| EPrj (e : SExp) (i : nat) (typ : Typ)
+| ECons (es : list SExp) (typ : Typ)
+| EIf (e e' e'' : SExp) (typ : Typ).
+
+(* getter of the type informations *)
+Definition typ_of e :=
+  match e with
+  | EVar _ ty => ty
+  | Enum _ => TZ
+  | ELet _ _ _ ty => ty
+  | EBin _ _ _ ty => ty
+  | EA _ _ ty => ty
+  | EPrj _ _ ty => ty
+  | ECons _ ty => ty
+  | EIf _ _ _ ty => ty
+  end.
+
+Lemma SExp_ind' : forall P : SExp -> Prop,
+    (forall (x : varE) ty, P (EVar x ty)) ->
+    (forall (x : Z), P (Enum x)) ->
+    (forall (x : varE) (e : SExp) ty, P e -> forall e' : SExp, P e' -> P (ELet x e e' ty)) ->
+    (forall (op : SOp) (e1 : SExp) ty, P e1 -> forall e2 : SExp, P e2 -> P (EBin op e1 e2 ty)) ->
+    (forall (x : varA) (e : SExp) ty, P e -> P (EA x e ty)) ->
+    (forall (e : SExp) ty, P e -> forall i : nat, P (EPrj e i ty)) ->
+    (forall (es : list SExp) ty, List.Forall P es -> P (ECons es ty)) ->
+    (forall (e : SExp) ty, P e -> forall e' : SExp, P e' -> forall e'' : SExp, P e'' -> P (EIf e e' e'' ty)) ->
+    forall e : SExp, P e.
+Proof.
+  intros; revert e.
+  refine (fix rec (e : SExp) := 
+    match e return P e with
+    | EVar x _ => H _ _
+    | Enum x => H0 _
+    | ELet x e e' _ => H1 _ _ _ (rec _) _ (rec _)
+    | EBin op e1 e2 _ => H2 _ _ _ (rec _) _ (rec _)
+    | EA x e _ => H3 _ _ _ (rec _)
+    | EPrj e i _ => H4 _ _ (rec _) _
+    | ECons es _ => 
+      let fix rec2 (es : list SExp) : List.Forall P es :=
+          match es return List.Forall P es with
+          | nil => List.Forall_nil _
+          | (e :: es')%list => List.Forall_cons _ (rec e) (rec2 es')
+          end in
+      H5 _ _ (rec2 es)
+    | EIf e e' e'' _ => H6 _ _ (rec _) _ (rec _) _ (rec _)
+    end).
+Qed.
+
+(* user defined functions *)
+Inductive Func := F (params : list varE) (body : SExp).
+
+(* array expressions *)
+Inductive AE :=
+  ALet (va : varA) (sk : name) (fs : list Func) (vas : list varA) (ea : AE)
+| ARet (va : varA).
+
+(* scalar/array values*)
+Inductive SVal : Set :=
+| VB (b : bool) | VZ (n : Z) | VTup (vs : list SVal).
+Record array :=
+  Arr {len_of : nat; dim_of : nat; arr_of : list SVal}.
+
+(* environments for variables *)
 Definition AEnv (A : Type) := Env varA A _.
 Definition SEnv (A : Type) := Env varE A _.
 
+(* eval environment, var -> val *)
 Notation AEnv_eval := (AEnv (option array)).
 Notation SEnv_eval := (SEnv (option SVal)).
 
@@ -96,164 +162,293 @@ Definition op_denote (op : SOp) (v1 v2 : SVal) :=
   | Blt => match v1, v2 with VZ v1, VZ v2 => Some (VB (v1 <? v2)) | _, _ => None end
   end%Z.
 
-Section EvalScalarExpr.
-Variable aenv : AEnv_eval.
+Section Semantics.
+  Variable aenv : AEnv_eval.
 
-Inductive abort := AB.
+  Inductive abort := AB.
 
-Inductive evalSE : (SEnv_eval) -> SExp -> SVal + abort -> Prop :=
-| EvalSE_var senv sx v :
-    senv sx = Some v -> evalSE senv (EVar sx) (inl v)
-| EvalSE_elet senv sx e1 e2 v1 v2 :
-    evalSE senv e1 (inl v1) ->
-    evalSE (upd_opt senv sx v1) e2 v2 ->
-    evalSE senv (ELet sx e1 e2) v2
-| EvalSE_EBin senv op e1 e2 v1 v2 v :
-    evalSE senv e1 (inl v1) ->
-    evalSE senv e2 (inl v2) ->
-    op_denote op v1 v2 = Some v ->
-    evalSE senv (EBin op e1 e2) (inl v)
-| EvalSE_EA_safe senv varA va e ix :
-    evalSE senv e (inl (VZ ix)) ->
-    aenv varA = Some va ->
-    (0 <= ix)%Z -> (ix < Z.of_nat (len va))%Z -> 
-    evalSE senv (EA varA e) (inl (List.nth (Z.to_nat ix) (arr va) (VZ 0)))
-| EvalSE_EA_abort senv varA va e ix :
-    evalSE senv e (inl (VZ ix)) ->
-    aenv varA = Some va ->
-    (ix < 0 \/ Z.of_nat (len va) < ix)%Z ->
-    evalSE senv (EA varA e) (inl (List.nth (Z.to_nat ix) (arr va) (VZ 0)))
-| EvalSE_EPrj senv e tup i :
-    evalSE senv e (inl (VTup tup)) ->
-    i < List.length (tup) ->
-    evalSE senv (EPrj e i) (inl (List.nth i tup (VZ 0)))
-| EvalSE_ECons senv es vs :
-    evalTup senv es (inl vs) ->
-    evalSE senv (ECons es) (inl (VTup vs))
-| EvalSE_Eif_true senv e e' e'' v :
-    evalSE senv e (inl (VB true)) ->
-    evalSE senv e' v ->
-    evalSE senv (EIf e e' e'') v
-| EvalSE_Eif_false senv e e' e'' v :
-    evalSE senv e (inl (VB false)) ->
-    evalSE senv e'' v ->
-    evalSE senv (EIf e e' e'') v
-with
-evalTup : (SEnv_eval) -> list SExp -> list SVal + abort -> Prop :=
-| EvalTup_nil senv : evalTup senv nil (inl nil)
-| EvalTup_cons senv e es v vs :
-    evalTup senv es (inl vs) ->
-    evalSE senv e (inl v) ->
-    evalTup senv (e :: es) (inl (v :: vs)).
+  (* semantics of scalar expressions *)
+  Inductive evalSE : Env varE (option SVal) _  -> SExp -> SVal + abort -> Prop :=
+  | EvalSE_var senv sx v ty :
+      senv sx = Some v -> evalSE senv (EVar sx ty) (inl v)
+  | EvalSE_Z senv n :
+      evalSE senv (Enum n) (inl (VZ n))
+  | EvalSE_elet senv sx e1 e2 v1 v2 ty:
+      evalSE senv e1 (inl v1) ->
+      evalSE (upd_opt senv sx v1) e2 v2 ->
+      evalSE senv (ELet sx e1 e2 ty) v2
+  | EvalSE_EBin senv op e1 e2 v1 v2 v ty:
+      evalSE senv e1 (inl v1) ->
+      evalSE senv e2 (inl v2) ->
+      op_denote op v1 v2 = Some v ->
+      evalSE senv (EBin op e1 e2 ty) (inl v)
+  | EvalSE_EA_safe senv varA va e ix ty:
+      evalSE senv e (inl (VZ ix)) ->
+      aenv varA = Some va ->
+      (0 <= ix)%Z -> (ix < Z.of_nat (len_of va))%Z -> 
+      evalSE senv (EA varA e ty) (inl (List.nth (Z.to_nat ix) (arr_of va) (VZ 0)))
+  | EvalSE_EA_abort senv varA va e ix ty :
+      evalSE senv e (inl (VZ ix)) ->
+      aenv varA = Some va ->
+      (ix < 0 \/ Z.of_nat (len_of va) < ix)%Z ->
+      evalSE senv (EA varA e ty) (inl (List.nth (Z.to_nat ix) (arr_of va) (VZ 0)))
+  | EvalSE_EPrj senv e tup i ty :
+      evalSE senv e (inl (VTup tup)) ->
+      i < List.length (tup) ->
+      evalSE senv (EPrj e i ty) (inl (List.nth i tup (VZ 0)))
+  | EvalSE_ECons senv es vs ty :
+      evalTup senv es (inl vs) ->
+      evalSE senv (ECons es ty) (inl (VTup vs))
+  | EvalSE_Eif_true senv e e' e'' v ty :
+      evalSE senv e (inl (VB true)) ->
+      evalSE senv e' v ->
+      evalSE senv (EIf e e' e'' ty) v
+  | EvalSE_Eif_false senv e e' e'' v ty :
+      evalSE senv e (inl (VB false)) ->
+      evalSE senv e'' v ->
+      evalSE senv (EIf e e' e'' ty) v
+  with
+  evalTup : (SEnv_eval) -> list SExp -> list SVal + abort -> Prop :=
+  | EvalTup_nil senv : evalTup senv nil (inl nil)
+  | EvalTup_cons senv e es v vs :
+      evalTup senv es (inl vs) ->
+      evalSE senv e (inl v) ->
+      evalTup senv (e :: es) (inl (v :: vs)).
 
-Fixpoint bind_vars (xs : list varE) (vs : list SVal) :=
-  match xs, vs with
-  | nil, nil => Some emp_opt
-  | (x :: xs), (v :: vs) =>
-    match bind_vars xs vs with
-    | None => None 
-    | Some bnd => Some (upd_opt bnd x v)
-    end
-  | _, _ => None
-  end.
+  (* semantics of functions *)
+  Fixpoint bind_vars (xs : list varE) (vs : list SVal) :=
+    match xs, vs with
+    | nil, nil => Some emp_opt
+    | (x :: xs), (v :: vs) =>
+      match bind_vars xs vs with
+      | None => None 
+      | Some bnd => Some (upd_opt bnd x v)
+      end
+    | _, _ => None
+    end.
 
-Inductive evalFunc : list SVal -> Func -> SVal + abort -> Prop :=
-| EvalFunc_app xs vs e v bnd : 
-    bind_vars xs vs = Some bnd ->
-    evalSE bnd e v ->
-    evalFunc vs (F xs e) v.
-End EvalScalarExpr.
+  Inductive evalFunc : list SVal -> Func -> SVal + abort -> Prop :=
+  | EvalFunc_app xs vs e v bnd : 
+      bind_vars xs vs = Some bnd ->
+      evalSE bnd e v ->
+      evalFunc vs (F xs e) v.
 
-Variable eval_skel : AEnv_eval -> name -> list Func -> list varA -> array + abort -> Prop.
+  Variable eval_skel : AEnv_eval -> name -> list Func -> list varA -> array + abort -> Prop.
+  
+  Inductive evalAE : AEnv_eval -> AE -> array + abort -> Prop :=
+  | EvalAE_ret aenv ax v :
+      aenv ax = Some v -> evalAE aenv (ARet ax) (inl v)
+  | EvalAE_alet (aenv : AEnv_eval) ax skl fs axs e2 v1 v2 :
+      eval_skel aenv skl fs axs (inl v1) ->
+      evalAE (upd_opt aenv ax v1) e2 v2 ->
+      evalAE aenv (ALet ax skl fs axs e2) v2.
+End Semantics.
 
-Inductive evalAE : AEnv_eval -> AE -> array + abort -> Prop :=
-| EvalAE_ret aenv ax v :
-    aenv ax = Some v -> evalAE aenv (ARet ax) (inl v)
-| EvalAE_alet (aenv : AEnv_eval) ax skl fs axs e2 v1 v2 :
-    eval_skel aenv skl fs axs (inl v1) ->
-    evalAE (upd_opt aenv ax v1) e2 v2 ->
-    evalAE aenv (ALet ax skl fs axs e2) v2.
 Require GPUCSL.
 Module G := GPUCSL.
 Require Skel_lemma.
 Module S := Skel_lemma.
 
-Section compile.
-  Import Lang.
-  Open Scope string_scope.
+Section typing_rule.
+  Definition ty_of_SOp (op : SOp) : list Typ -> option Typ :=
+    match op with
+    | Top.Eplus => fun tys =>
+                     match tys with
+                     | TZ :: TZ :: nil => Some TZ
+                     | _ => None
+                     end
+    | Top.Emax => fun tys =>
+                    match tys with
+                    | TZ :: TZ :: nil => Some TZ
+                    | _ => None
+                    end
+    | Top.BEq => (fun tys => 
+                   match tys with
+                   | ty1 :: ty2 :: nil => if STyp_eq_dec ty1 ty2 then Some TBool else None
+                   | _ => None
+                  end)
+    | Top.Blt => fun tys =>
+                   match tys with
+                   | TZ :: TZ :: nil => Some TBool
+                   | _ => None
+                   end
+    end.
 
-  Notation SVEnv := (Env varE (list exp) _).
+  Fixpoint typing (atyenv : Env varA (option Typ) _) (styenv : Env varE (option Typ) _) (e : SExp) : option (SExp * Typ) :=
+    match e with
+    | EVar x _ => match styenv x with Some ty => Some (EVar x ty, ty) | None => None end
+    | Top.Enum n => Some (Top.Enum n, TZ)
+    | ELet x e1 e2 _ =>
+      match typing atyenv styenv e1 with
+      | Some (e1, tye1) =>
+        match typing atyenv (upd_opt styenv x tye1) e2 with
+        | Some (e2, tye2) =>
+          Some (ELet x e1 e2 tye2, tye2)
+        | None => None
+        end
+      | None => None
+      end
+    | EBin op e1 e2 _ =>
+      match typing atyenv styenv e1 with
+      | Some (e1, tye1) =>
+        match typing atyenv styenv e2 with
+        | Some (e2, tye2) =>
+          match ty_of_SOp op (tye1 :: tye2 :: nil) with
+          | Some tyres => Some (EBin op e1 e2 tyres, tyres)
+          | None => None
+          end
+        | None => None
+        end
+      | None => None
+      end
+    | EA xa i _ =>
+      match atyenv xa with
+      | Some aty => Some (EA xa i aty, aty)
+      | None => None
+      end
+    | EPrj e i _ =>
+      match typing atyenv styenv e with
+      | Some (e, ty) => 
+        match ty with
+        | TTup tys => if lt_dec i (length tys) then Some (EPrj e i (nth i tys TZ), nth i tys TZ) else None
+        | _ => None
+        end
+      | None => None
+      end
+    | ECons es _ =>
+      match fold_right (fun e tys => match typing atyenv styenv e with
+                               | None => None
+                               | Some (e, ty) =>
+                                 match tys with
+                                 | None => None
+                                 | Some (es, tys) => Some (e :: es, ty :: tys)
+                                 end
+                        end) (Some (nil, nil)) es with
+      | None => None
+      | Some (es, tys) => Some (ECons es (TTup tys), (TTup tys))
+      end
+    | EIf e1 e2 e3 _ =>
+      match typing atyenv styenv e1,
+            typing atyenv styenv e2,
+            typing atyenv styenv e3 with
+      | Some (e1, TBool), Some (e2, ty2), Some (e3, ty3) =>
+        if STyp_eq_dec ty2 ty3 then Some (EIf e1 e2 e3 ty2, ty2)
+        else None
+      | _, _, _ => None
+      end
+    end.
+End typing_rule.
 
-  Definition M a := nat -> (option a * nat).
+Section codegen.
+  Definition M a := nat -> ((a + string) * nat).
 
   Definition bind_opt A B (e : M A) (f : A -> M B) : M B:=
     fun n => 
       match e n with
-      | (None, n) => (None, n)
-      | (Some v, n) => f v n
+      | (inr msg, n) => (inr msg, n)
+      | (inl v, n) => f v n
       end.
 
-  Infix ">>=" := (bind_opt _ _) (at level 70).
-
-  Definition ret {A} (x : A) : M A := fun n => (Some x, n).
-  Definition fail {A} : M A  := fun n => (None, n).
+  Definition ret {A} (x : A) : M A := fun n => (inl x, n).
+  Definition fail {A} (msg : string): M A  := fun n => (inr msg, n).
   
-  Definition get : M nat := fun n => (Some n, n).
-  Definition set n : M unit := fun _ => (Some tt, n).
+  Definition get : M nat := fun n => (inl n, n).
+  Definition set n : M unit := fun _ => (inl tt, n).
+End codegen.
 
-Definition freshes dim : M (list var) :=
-  let fix f dim n :=
-      match dim with
-      | O => ret nil
-      | S dim =>
-        f dim n >>= fun fs =>
-        ret (Var ("l" ++ S.nat_to_string n ++ "_" ++ S.nat_to_string dim) :: fs)
-      end in
-  get >>= fun n =>
-  set (n + 1) >>= fun _ =>
-  f dim n.
+Infix ">>=" := (bind_opt _ _) (at level 70).
+
+Section compiler.
+  (* typing environment of array *)
+  Variable atyenv : Env varA Typ _.
+  (* environment of variables of array in the generated code *)
+  Variable avarenv : Env varA (list var) _.
+
+  Fixpoint string_of_ty ty : string :=
+    match ty with
+    | TBool => "Bool"
+    | TZ => "Z"
+    | TTup ls => "(" ++ fold_right (fun x y => string_of_ty x ++ y) ")" ls
+    end%string.
+
+  Fixpoint len_of_ty ty : nat :=
+    match ty with
+    | TBool | TZ => 1
+    | TTup ls => fold_right (fun x y => len_of_ty x + y) 0 ls
+    end.
   
-  Notation ATyEnv := (Env varA nat _).
-  Notation AVarEnv := (Env varA (list var) _).
+  Fixpoint len_until_i tys i : nat :=
+    fold_right (fun ty n => len_of_ty ty + n) 0 (firstn i tys).
+  
+  Fixpoint len_at_i (tys : list Typ) i : nat :=
+    len_of_ty (nth i tys TZ).
+  
+  Import Lang.
+  Open Scope string_scope.
 
-  Variable atyenv : ATyEnv.
-  Variable avarenv : AVarEnv.
+  Notation SVEnv := (Env varE (list var) _).
 
+  Definition freshes dim : M (list var) :=
+    let fix f dim n :=
+        match dim with
+        | O => ret nil
+        | S dim =>
+          f dim n >>= fun fs =>
+           ret (Var ("l" ++ S.nat_to_string n ++ "_" ++ S.nat_to_string dim) :: fs)
+        end in
+    get >>= fun n =>
+    set (n + 1) >>= fun _ =>
+    f dim n.
+
+  (* compiler of scalar expressions *)
   Fixpoint compile_sexp (se : SExp) (env : SVEnv) : M (cmd * list exp) := match se with
-    | EVar v => ret (Cskip, env v)
+    | EVar v _ => ret (Cskip, S.vars2es (env v))
     | Top.Enum z => ret (Cskip, Enum z :: nil)
-    | ELet x e1 e2 =>
+    | ELet x e1 e2 _ =>
       compile_sexp e1 env >>= fun ces1 => 
       let (c1, es1) := ces1 in
       let dim := length es1 in
       freshes dim >>= fun xs =>
-      compile_sexp e2 (upd env x (S.vars2es xs)) >>= fun ces2 => 
+      compile_sexp e2 (upd env x xs) >>= fun ces2 => 
       let (c2, es2) := ces2 in
       ret (c1 ;; S.read_tup xs es1 ;; c2, es2)
-    | EBin op e1 e2 => 
+    | EBin op e1 e2 _ => 
       compile_sexp e1 env >>= fun ces1 =>
       let (c1, es1) := ces1 in
       compile_sexp e2 env >>= fun ces2 =>
       let (c2, es2) := ces2 in
       match es1, es2 with
       | e1 :: nil, e2 :: nil => ret (c1 ;; c2, e1 +C e2 :: nil)
-      | _, _ => fail
+      | _, _ => fail ""
       end
-    | EA va e =>
+    | EA va e _ =>
       compile_sexp e env >>= fun ces =>
       let (c, es) := ces in
       let aty := atyenv va in
       let aname := avarenv va in
-      freshes aty >>= fun xs =>
+      freshes (len_of_ty aty) >>= fun xs =>
       match es with
       | i :: nil => ret (c ;; S.gen_read Gl xs (S.vars2es aname) i, S.vars2es xs)
-      | _ => fail
+      | _ => fail ""
       end
-    | EPrj e i =>
-      compile_sexp e env >>= fun ces =>
-      let (c, es) := ces in
-      if lt_dec i (length es) then ret (Cskip, nth i es 0%Z :: nil) else fail
-    | ECons es => 
+    | EPrj e i ty =>
+      match typ_of e with
+      | TBool | TZ => fail ""
+      | TTup tys => 
+        let off := len_until_i tys i in
+        let l := len_at_i tys i in
+        compile_sexp e env >>= fun ces =>
+        let (c, es) := ces in
+        if le_dec (off + l) (len_of_ty (TTup tys)) then
+          ret (Cskip, firstn l (skipn off es))
+        else fail ("overflow the index " ++ S.nat_to_string i ++ " of tuple:
+" ++               "type of tuple: " ++ string_of_ty ty ++
+
+                   "expected length = " ++ S.nat_to_string (len_of_ty ty) ++ "
+" ++
+                   "actual length = " ++ S.nat_to_string off ++ " + " ++ S.nat_to_string l)
+      end
+    | ECons es _ => 
       let fix compile_sexps (es : list SExp) env : M (cmd * list exp) :=
           match es with
           | nil => ret (Cskip, nil)
@@ -265,7 +460,7 @@ Definition freshes dim : M (list var) :=
             ret (c ;; c', ge ++ ges)
           end in
       compile_sexps es env
-    | EIf e1 e2 e3 => 
+    | EIf e1 e2 e3 _ => 
       compile_sexp e1 env >>= fun ces1 => 
       let (c1, e1) := ces1 in
       compile_sexp e2 env >>= fun ces2 =>
@@ -277,17 +472,238 @@ Definition freshes dim : M (list var) :=
       match e1 with
       | e :: nil =>
         ret (Cif (e == 0%Z) (c2 ;; S.read_tup xs e2) (c3 ;; S.read_tup xs e3), S.vars2es xs)
-      | _ => fail
+      | _ => fail ""
       end
     end%list.
-  
-  Coercion VarE : string >-> varE.
-  Coercion EVar : varE >-> SExp.
-  Coercion Top.Enum : Z >-> SExp.
+End compiler.
 
-  Eval cbv in 
-      compile_sexp (
-        ELet "x" (ECons ((1%Z : SExp)  :: (2%Z : SExp) :: nil)) (
-        ELet "y" (ECons ((3%Z : SExp)  :: (4%Z : SExp) :: nil)) (
-        ELet "z" (ECons (("x" : SExp) :: ("y" : SExp) :: nil)) (
-        EPrj "z" 0)))) (emp_def nil) 0.
+Section TestCompiler.
+  Definition EVar' (x : varE) := EVar x TZ.
+  Definition ELet' (x : varE) (e e' : SExp)  := ELet x e e' TZ.
+  Definition EBin' (op : SOp) (e1 e2 : SExp) := EBin op e1 e2 TZ.
+  Definition EA' (x : varA) (e : SExp) (typ : Typ) := EA x e TZ.
+  Definition EPrj' (e : SExp) (i : nat) := EPrj e i TZ.
+  Definition ECons' (es : list SExp) := ECons es TZ.
+  Definition EIf' (e e' e'' : SExp) := EIf e e' e'' TZ.
+  
+  Open Scope string_scope.
+
+  Coercion VarE : string >-> varE.
+  Coercion Top.Enum : Z >-> SExp.
+  Coercion EVar' : varE >-> SExp.
+
+  Definition test1 :=
+    typing emp_opt emp_opt(
+             ELet' "x" (ECons' ((1%Z : SExp)  :: (2%Z : SExp) :: nil)) (
+                     ELet' "y" (ECons' ((3%Z : SExp)  :: (4%Z : SExp) :: nil)) (
+                             ELet' "z" (ECons' (("x" : SExp) :: ("y" : SExp) :: nil)) ( 
+                                     EPrj' "z" 0)))).
+  
+  Eval cbv in test1.
+  Eval cbv in (match test1 with Some (t, _) => Some (compile_sexp (emp_def TZ) (emp_def nil) t (emp_def nil) 0) | None => None end).
+  
+End TestCompiler.
+
+Section CorrectnessProof.
+  Import Skel_lemma.
+  (* the set of free variables *)
+  Variable free_avs : list varA.
+  (* the evaluation environment *)
+  Variable aeval_env : Env varA (option array) _.
+  (* the typing environment *)
+  Variable aty_env : Env varA Typ _.
+  (* the variable mapping environment between source and dest. *)
+  Variable avar_env : Env varA (list var) _ .
+  
+  (* free variables lists does not have any duplicated variables *)
+  Hypothesis nodup_favs : NoDup free_avs.
+  
+  (* source lang. values -> dest. lang. values *)
+  Fixpoint vs_of_sval sval : list Z :=
+    match sval with
+    | VB b => (if b then 1%Z else 0%Z) :: nil
+    | VZ z => z :: nil
+    | VTup vs => fold_right (fun v vs => vs_of_sval v ++ vs) nil vs
+    end%list.
+
+  (* precondition of free variable arrays *)
+  Fixpoint assn_of_avs (favs : list varA) :=
+    match favs with
+    | nil => emp
+    | x_a :: avs =>
+      match aeval_env x_a with
+      | None => FalseP
+      | Some a =>
+        S.is_tuple_array_p (S.es2gls (S.vars2es (avar_env x_a))) (len_of a) (fun i => vs_of_sval (nth i (arr_of a) (VZ 0))) 0 1 **
+        assn_of_avs avs
+      end
+    end.
+
+  (* (* the set of free variables of scalar exp *) *)
+  (* Variable free_svs : list varE. *)
+  (* (* the evaluation environment of scalar exp *) *)
+  (* Variable seval_env : Env varE (option SVal) _. *)
+  (* (* the typing environment *) *)
+  (* Variable sty_env : Env varE Typ _. *)
+  (* (* the variable mapping environment between source and dest. *) *)
+  (* Variable svar_env : Env varE (list var) _ . *)
+
+  (* preconditions of scalar variables *)
+  Fixpoint assn_of_svs (seval_env : Env varE (option SVal) _) (svar_env : Env varE (list var) _)  (fsvs : list varE) :=
+    match fsvs with
+    | nil => emp
+    | x_e :: svs =>
+      match seval_env x_e with
+      | Some v => !(vars2es (svar_env x_e) ==t vs_of_sval v) ** assn_of_svs seval_env svar_env svs
+      | None => FalseP
+      end
+    end.
+  
+  Variable ntrd : nat.
+  Variable tid : Fin.t ntrd.
+  Variable BS : nat -> Vector.t assn ntrd * Vector.t assn ntrd.
+  
+  Definition equiv_ls {A : Type} (ls1 ls2 : list A) := (incl ls1 ls2) /\ (incl ls2 ls1).
+
+  Require Import Recdef.
+  Lemma remove_length {A : Type} {eqt : eq_type A} (xs : list A) x:
+    length (remove eq_dec x xs) <= length xs.
+  Proof.
+    induction xs; simpl; try omega.
+    destruct eq_dec; simpl; try omega.
+  Qed.
+  
+  Function uniq {A} {eqt : eq_type A} (xs : list A) {measure length xs} :=
+    match xs with
+    | nil => nil
+    | x :: xs => x :: uniq (remove eq_dec x xs)
+    end.
+  Proof.
+    intros; simpl.
+    lets: (>> remove_length xs0 x); simpl in *; try omega.
+  Defined.
+  Arguments uniq {A eqt} xs : rename.
+
+  Lemma remove_incl {A} {eqt : eq_type A} x (xs : list A) :
+    incl (remove eq_dec x xs) xs.
+  Proof.
+    induction xs; unfold incl in *; simpl; eauto.
+    destruct (eq_dec _ _); substs; simpl in *; jauto.
+    intros ? [? | ?]; eauto.
+  Qed.
+  
+  Lemma uniq_incl {A} {eqt : eq_type A} (xs : list A) :
+    incl (uniq xs) xs.
+  Proof.
+    functional induction (uniq xs).
+    - unfold incl; eauto.
+    - unfold incl in *; simpl.
+      intros ? [? | ?]; eauto.
+      forwards* : IHl.
+      forwards* : remove_incl.
+  Qed.
+
+  Lemma uniq_no_dup {A} {eqt : eq_type A} (xs : list A) :
+    NoDup (uniq xs).
+  Proof.
+    functional induction (uniq xs).
+    - constructor.
+    - constructor; eauto.
+      intros Hc.
+      forwards*: uniq_incl; unfold incl in *; eauto.
+      apply H in Hc; forwards*: remove_In; eauto.
+  Qed.
+
+  Import scan_lib.
+
+  Fixpoint free_sv' (e : SExp) :=
+    match e with
+    | EVar v _ => v :: nil
+    | Enum _   => nil
+    | ELet x e1 e2 _ => 
+      free_sv' e1 ++ remove eq_dec x (free_sv' e2)
+    | EBin _ e1 e2 _ => free_sv' e1 ++ free_sv' e2
+    | EA _ e _ => free_sv' e
+    | EPrj e _ _ => free_sv' e
+    | ECons es _ => fold_right (fun e xs => free_sv' e ++ xs) nil es
+    | EIf e e' e'' _ => free_sv' e ++ free_sv' e' ++ free_sv' e''
+    end.
+
+  Fixpoint free_av' (e : SExp) :=
+    match e with
+    | EVar v _ => nil
+    | Enum _   => nil
+    | ELet x e1 e2 _ => 
+      free_av' e1 ++ free_av' e2
+    | EBin _ e1 e2 _ => free_av' e1 ++ free_av' e2
+    | EA x e _ => x :: free_av' e
+    | EPrj e _ _ => free_av' e
+    | ECons es _ => fold_right (fun e xs => free_av' e ++ xs) nil es
+    | EIf e e' e'' _ => free_av' e ++ free_av' e' ++ free_av' e''
+    end.
+
+  Definition free_sv e := uniq (free_sv' e).
+  Definition free_av e := uniq (free_av' e).
+
+  Lemma compile_ok (se : SExp) (seval_env : Env varE (option SVal) _)
+        (svar_env : Env varE (list var) _) (n m : nat)
+        (sv : SVal) c es :
+    evalSE aeval_env seval_env se (inl sv) ->
+    compile_sexp aty_env avar_env se svar_env n =  (inl (c, es), m) ->
+    CSL BS tid
+        (!(assn_of_svs seval_env svar_env (free_sv se)) **
+          (assn_of_avs (free_av se)))
+        c
+        (!(assn_of_svs seval_env svar_env (free_sv se)) **
+          (assn_of_avs (free_av se)) ** !(es ==t vs_of_sval sv)).
+  Proof.
+    revert se seval_env svar_env n m sv c es.
+    induction se using SExp_ind'; simpl;
+    introv.
+    - intros Heval Hcompile.
+      unfold ret in Hcompile; inversion Hcompile; substs.
+      inversion Heval; substs; simpl in *.
+      eapply Hforward; eauto using rule_skip.
+      intros; sep_split; sep_split_in H; repeat sep_cancel.
+      destruct (seval_env x); sep_split_in H; sep_split; eauto.
+      + inverts H1; sep_normal_in HP; sep_split_in HP; eauto.
+      + destruct HP.
+      (* assert (Hin : In x ) by (destruct Heq1; unfold incl in *; simpl in *; eauto). *)
+      
+      (* Lemma assn_of_svs_in seval_env svar_env x fv v : *)
+      (*   In x fv -> *)
+      (*   seval_env x = Some v -> *)
+      (*   !(assn_of_svs seval_env svar_env fv) |= !(S.vars2es (svar_env x) ==t vs_of_sval v). *)
+      (* Proof. *)
+      (*   induction fv; simpl in *; destruct 1; substs; intros Heq. *)
+      (*   - rewrite Heq. *)
+      (*     intros. *)
+      (*     sep_rewrite_in pure_star H; sep_rewrite_in pure_pure H. *)
+      (*     sep_split_in H; sep_split; eauto. *)
+      (*   - destruct (seval_env a); [|intros ? ? [? []]]. *)
+      (*     intros stk h H'. *)
+      (*     sep_rewrite_in pure_star H'; sep_rewrite_in pure_pure H'. *)
+      (*     sep_split_in H'. *)
+      (*     apply IHfv; eauto; sep_split; eauto. *)
+      (* Qed. *)
+
+      (* forwards: (>>assn_of_svs_in s (emp_ph loc)); eauto. *)
+      (* sep_split; eauto using emp_emp_ph. *)
+      (* sep_split_in H0; eauto. *)
+
+    - intros _; introv Heval Hcompile.
+      inversion Hcompile; substs.
+      eapply Hforward; [apply rule_skip|].
+      intros; sep_split; sep_split_in H; eauto.
+      inversion Heval; substs.
+      simpl; sep_split; eauto using emp_emp_ph; unfold_conn; simpl; auto.
+    - introv Heval Hcompile.
+      unfold bind_opt in Hcompile.
+      destruct (compile_sexp _ _ se1 _ _) as [[(cs1 & es1) | ?] n'] eqn:Hceq1; [|inversion Hcompile].
+      destruct (freshes (length es1) _) as [[fvs1 | ?] n''] eqn:Hfeq1; [|inversion Hcompile].
+      destruct (compile_sexp _ _ se2 _ _) as [[(cs2 & es2) | ?] n'''] eqn:Hceq2; [|inversion Hcompile].
+      inverts Hcompile; substs.
+      inverts Heval; substs.
+      
+      forwards*: IHse1.
+      
